Some progress making simplifications

src/Spec/Proc.v
@@ -33,14 +33,14 @@ Section Dynamics.
   (** First, we define semantics of running programs with halting (without the
   effect of a crash or recovery) *)
 
-  Fixpoint exec T (p: proc T) : relation State T :=
+  Fixpoint exec {T} (p: proc T) : relation State T :=
     match p with
     | Ret v => pure v
     | Prim op => step op
     | Bind p p' => v <- exec p; exec (p' v)
     end.
 
-  Fixpoint exec_crash T (p: proc T) : relation State unit :=
+  Fixpoint exec_crash {T} (p: proc T) : relation State unit :=
     match p with
     | Ret v => pure tt
     | Prim op => pure tt + (step op;; pure tt)
@@ -50,13 +50,13 @@ Section Dynamics.
                      (exec_crash (p' v)))
     end.
 
-  Definition exec_recover R (rec: proc R) : relation State R :=
-    seq_star (crash_step;; exec_crash rec);;
-             (crash_step;; exec rec).
+  Definition exec_recover {R} (rec: proc R) : relation State R :=
+    seq_star (exec_crash rec;; crash_step);;
+             exec rec.
 
   (* recovery execution *)
-  Definition rexec T R (p: proc T) (rec: proc R) : relation State R :=
-      exec_crash p;; exec_recover rec.
+  Definition rexec {T R} (p: proc T) (rec: proc R) : relation State R :=
+      exec_crash p;; crash_step;; exec_recover rec.
 
 End Dynamics.
 
