src/Helpers/RelationAlgebra.v
@@ -17,10 +17,6 @@ Section OutputRelations.
     relation T2 :=
     fun x z o2 => exists o1 y, r1 x y o1 /\ (r2 o1) y z o2.
 
-  Definition seq {T1 T2} (r1: relation T1) (r2: relation T2)
-    : relation T2 :=
-    and_then r1 (fun _ => r2).
-
   Definition fmap T1 T2 (f: T1 -> T2) (r:relation T1) : relation T2 :=
     fun x y o => exists o0, r x y o0 /\ o = f o0.
 
@@ -32,6 +28,8 @@ Section OutputRelations.
 
   Definition rel_or T (r1 r2: relation T) : relation T :=
     fun x y o => r1 x y o \/ r2 x y o.
+
+  Infix "+" := rel_or.
 
   Inductive seq_star `(r: relation T) : relation T :=
   | seq_star_refl : forall x o,
@@ -63,8 +61,8 @@ Section OutputRelations.
   Definition requiv {T} (r1 r2: relation T) :=
     forall x y o, r1 x y o <-> r2 x y o.
 
-  Infix "--->" := rimpl (at level 40, no associativity).
-  Infix "<--->" := requiv (at level 40, no associativity).
+  Infix "--->" := rimpl (at level 60, no associativity).
+  Infix "<--->" := requiv (at level 60, no associativity).
 
   Global Instance rimpl_requiv_sub : subrelation (requiv (T:=T)) rimpl :=
     ltac:(firstorder).
@@ -73,7 +71,8 @@ Section OutputRelations.
     RelInstance.
 
   Hint Unfold Proper respectful pointwise_relation : t.
-  Hint Unfold seq and_then rel_or pure : t.
+  Hint Unfold Basics.flip Basics.impl : t.
+  Hint Unfold and_then rel_or pure : t.
 
   Ltac t :=
     autounfold with t;
@@ -90,34 +89,20 @@ Section OutputRelations.
                   H': ?r ?x ?y ?o |- _ ] =>
              add_hypothesis (H x y o H')
            | _ => progress propositional
-           | _ => eauto 10
+           | _ => solve [ eauto 10 ]
+           | [ H: _ \/ _  |- _ ] => destruct H
         end.
-
-  Global Instance seq_respects_equiv :
-    Proper (requiv ==> requiv ==> requiv) (seq (T1:=T1) (T2:=T2)).
-  Proof.
-    t.
-  Qed.
-
-  Global Instance seq_respects_impl :
-    Proper (rimpl ==> rimpl ==> rimpl) (seq (T1:=T1) (T2:=T2)).
-  Proof.
-    t.
-  Qed.
 
   Global Instance or_respects_equiv :
     Proper (requiv ==> requiv ==> requiv) (rel_or (T:=T)).
   Proof.
     t.
-    (intuition idtac); t.
-    (intuition idtac); t.
   Qed.
 
   Global Instance or_respects_impl :
     Proper (rimpl ==> rimpl ==> rimpl) (rel_or (T:=T)).
   Proof.
     t.
-    (intuition idtac); t.
   Qed.
 
   Theorem rel_or_introl T (r1 r2: relation T) :
@@ -132,25 +117,10 @@ Section OutputRelations.
     t.
   Qed.
 
-  Theorem seq_assoc
-          `(r1: relation T1)
-          `(r2: relation T2)
-          `(r3: relation T3) :
-    seq (seq r1 r2) r3 <---> seq r1 (seq r2 r3).
-  Proof.
-    t.
-  Qed.
-
   Theorem bind_left_id T1 T2 (v:T1) (r: T1 -> relation T2) :
     and_then (pure v) r <---> r v.
   Proof.
     t.
-  Qed.
-
-  Theorem seq_left_id T1 T2 (v:T1) (r: relation T2) :
-    seq (pure v) r <---> r.
-  Proof.
-    unfold seq; apply bind_left_id.
   Qed.
 
   Theorem bind_assoc T1 T2 T3
@@ -163,17 +133,7 @@ Section OutputRelations.
     t.
   Qed.
 
-  Theorem bind_seq_assoc T1 T2 T3
-          (r1: relation T1)
-          (r2: T1 -> relation T2)
-          (r3: relation T3) :
-    seq (and_then r1 r2) r3 <--->
-             and_then r1 (fun v => seq (r2 v) r3).
-  Proof.
-    t.
-  Qed.
-
-  Theorem and_then_cong T1 T2 (r1 r1': relation T1) (r2 r2': T1 -> relation T2) :
+  Theorem and_then_impl_cong T1 T2 (r1 r1': relation T1) (r2 r2': T1 -> relation T2) :
     r1 ---> r1' ->
     (forall x, r2 x ---> r2' x) ->
     and_then r1 r2 ---> and_then r1' r2'.
@@ -186,18 +146,72 @@ Section OutputRelations.
     Proper (rimpl ==> pointwise_relation _ rimpl ==> rimpl) (and_then (T1:=T1) (T2:=T2)).
   Proof.
     unfold Proper, "==>"; intros.
-    apply and_then_cong; auto.
+    apply and_then_impl_cong; auto.
+  Qed.
+
+  Theorem and_then_equiv_cong T1 T2 (r1 r1': relation T1) (r2 r2': T1 -> relation T2) :
+    r1 <---> r1' ->
+    (forall x, r2 x <---> r2' x) ->
+    and_then r1 r2 <---> and_then r1' r2'.
+  Proof.
+    t.
+    specialize (H0 o1); t.
+    specialize (H0 o1); t.
+  Qed.
+
+  Global Instance and_then_respectful_equiv :
+    Proper (requiv ==> pointwise_relation _ requiv ==> requiv) (and_then (T1:=T1) (T2:=T2)).
+  Proof.
+    unfold Proper, "==>"; intros.
+    apply and_then_equiv_cong; auto.
+  Qed.
+
+  Hint Constructors seq_star.
+
+  Global Instance seq_star_respectful T :
+    Proper (rimpl ==> rimpl) (seq_star (T:=T)).
+  Proof.
+    t.
+    induction H0; eauto.
+  Qed.
+
+  Hint Constructors bind_star.
+
+  Global Instance bind_star_respectful T :
+    Proper (pointwise_relation _ rimpl ==> pointwise_relation _ rimpl) (bind_star (T:=T)).
+  Proof.
+    t.
+    induction H0; eauto.
+    specialize (H o1); eauto.
+  Qed.
+
+  Global Instance rimpl_equiv_proper T (r: relation T) :
+    Proper (requiv ==> Basics.flip Basics.impl) (rimpl r).
+  Proof.
+    t.
   Qed.
 
   Definition rimpl_refl T (r: relation T) : r ---> r := ltac:(reflexivity).
   Definition requiv_refl T (r: relation T) : r <---> r := ltac:(reflexivity).
+
+  Theorem bind_dist_r T1 T2 (r1 r2: relation T1) (r3: T1 -> relation T2) :
+    and_then (r1 + r2) r3 <---> (and_then r1 r3) + (and_then r2 r3).
+  Proof.
+    t.
+  Qed.
+
+  Theorem bind_dist_l T1 T2 (r1: relation T1) (r2 r3: T1 -> relation T2) :
+    and_then r1 (fun v => r2 v + r3 v) <---> and_then r1 r2 + and_then r1 r3.
+  Proof.
+    t.
+  Qed.
 
 End OutputRelations.
 
 Module RelationNotations.
   Infix "--->" := rimpl (at level 40, no associativity).
   Infix "<--->" := requiv (at level 40, no associativity).
-  Infix ";;" := seq (at level 21, left associativity).
+  Notation "p1 ;; p2" := (and_then p1 (fun _ => p2)) (at level 21, left associativity).
   Infix "+" := rel_or.
   Notation "x <- p1 ; p2" := (and_then p1 (fun x => p2))
                                (at level 60, right associativity).
